\documentclass[a4paper,10pt]{article}
\title{}
\author{}
\usepackage{graphicx} 
\parskip 7.2pt

\begin{document}
\maketitle
\begin{abstract}

We consider the family of trianges in the hyperbolic two dimensional space with
angles $\alpha, \beta, \gamma < \frac{\pi}{2}$ and test the Fangano orbits enclosed
in them. We try to find those whose orbits are in some sense 'maximal'. A question
arises as to what sense the maximum is measure since normalization not as simple as
the Euclidean case. We show that the area of the triangle is in may ways a good
normailzation factor and that maximizing the ratio between the length of the Fangano
orbit and the triangle's area makes sense.


\end {abstract}

\section{The equilateral case}

We use the above to derive the formula for the Fangano triangle length of the
equilateral hyperbolic triangle of edge length $a$.

Using the rule of cosines:

\begin{center}
$\frac{\cosh^2{a} - \cosh{a}}{\sinh^2{a}} = \cos{\alpha} = \frac{\cosh^2{\frac{a}{2}} - \cosh{\frac{x}{3}}}{\sinh^2{\frac{a}{2}}}$
\end{center}

And solving for x:

$ \cosh{\frac{x}{3}} = \cosh^2{\frac{a}{2}} - \sinh^2{\frac{a}{2}}\frac{\cosh^2{a} - \cosh{a}}{\sinh^2{a}} = $

$ \cosh{\frac{x}{3}} = \frac{1}{2}\left(\cosh{a}+1\right) - \frac{1}{2}\left(\cosh{a}-1\right)\frac{\cosh^2{a} - \cosh{a}}{\cosh^2{a} - 1} = $

$ \cosh{\frac{x}{3}} = \frac{1}{2}\left(\cosh{a}+1\right) - \frac{1}{2}\frac{\cosh{a}\left(\cosh{a}-1\right)}{\cosh{a} + 1} =$

$ \cosh{\frac{x}{3}} = \frac{\left(\cosh{a}+1\right)^{2} - \cosh{a}\left(\cosh{a}-1\right)}{2\cosh{a} + 2} =$

$ \cosh{\frac{x}{3}} = \frac{3\cosh{a}+1}{2\cosh{a} + 2} =$
$ \cosh{\frac{x}{3}} = \frac{3\cosh{a}+3}{2\cosh{a} + 2} - \frac{2}{2\cosh{a} + 2} = \frac{3}{2} - \frac{1}{\cosh{a} + 1}$

And so the length of the Fangano orbit is:

\begin{center}
$ 3acosh\left(\frac{3}{2} - \frac{1}{\cosh{a} + 1}\right)$
\end{center}

We easily deduce from the rule of cosines that the area of the Triangle is:


$ \pi - 3\alpha = \pi - 3acos\left(\frac{\cosh^2{a} - \cosh{a}}{\sinh^2{a}}\right) = \pi - 3acos\left(\frac{\cosh^2{a} - \cosh{a}}{\cosh^2{a} - 1}\right) = \pi - 3acos\left(\frac{\cosh{a}}{\cosh{a} + 1}\right) = $

\begin{center}

$ \pi - 3acos\left(1 - \frac{1}{\cosh{a} + 1}\right) $
\end{center}

And also:

\begin{center}

$ \cos{\alpha} = 1 - \frac{1}{\cosh{a}+1} $
\end{center}

The circumference is, naturally $3a$.


It is thus natural to ask, which $\alpha$ maximizes the ratio $r$ between the
Fangano orbit length and the area of the triangle.
\begin {center}

$\left(\frac{  3acosh\left(\frac{1}{2} + \cos{\alpha} \right)}{\pi - 3\alpha} \right)' = 3\frac{-\sin{\alpha}\left(\left(\frac{1}{2}  +\cos{\alpha}\right)^2 + 1\right)^{-\frac{1}{2}} +3acosh\left(\frac{1}{2}+\cos{\alpha}\right) }{\left( \pi-3\alpha \right)^2}$

\end{center}




\section{The general case}

We will skip showing that the Fangano orbit is indeed the triangle connecting the
bases of the heights and from now on refer to such inner triangles when using the
term Fangano orbit.

Let us first find an explicit formula for the length of the Fangano orbit,
starting with the length of the perpendicular $p_c$ to $c$ leaving $C$.
By the hyperbolic pythagorian rule, the following holds for every triangle:

\begin{center}
$ (*) \cosh{a} = \cosh{c_a}\cosh{p_c}$

$ (**) \cosh{b} = \cosh{c_b}\cosh{p_c}$
\end{center}

We substitue for:

\begin{center}
$ \cosh{c_a} = \cosh{c - c_b} = \cosh{c}\cosh{c_b} - \sinh{c}\sinh{c_b} $
\end{center}

in $(*)$ and recieve: 

\begin{center}
$\cosh{a} = \left(\cosh{c}\cosh{c_b} - \sinh{c}\sinh{c_b}\right)\cosh{p_c} =$


\end{center}


Dividing by $(**)$:

$\frac{\cosh{a}}{\cosh{b}} = \frac{\cosh{c}\cosh{c_b} - \sinh{c}\sinh{c_b}}{\cosh{c_b}} =$
$\cosh{c} - \frac{\sinh{c}\sinh{c_b}}{\cosh{c_b}} $

We get:

\begin{center}
$\tanh{c_b} = \frac{\cosh{c}\cosh{b} - \cosh{a}}{\cosh{b}\sinh{c}} $

$\cosh{c_b} = \frac{1}{\sqrt{1-\tanh^2{c_b}}} = \frac{1}{\sqrt{1 - \left(\frac{\cosh{c}\cosh{b} - \cosh{a}}{\cosh{b}\sinh{c}}\right)^2}} = $

$ \frac{\cosh{b}\sinh{c}}{\sqrt{\cosh^2{b}\sinh^2{c} - \left(\cosh{c}\cosh{b} - \cosh{a}\right)^2}} =$

$ \frac{\cosh{c}\cosh{b}}{\sqrt{2\cosh{a}\cosh{b}\cosh{c} - \cosh^2{b} - \cosh^2{a}}}$

\end{center}

and in the same way:
\begin{center}
$\tanh{b_c} = \frac{\cosh{b}\cosh{c} - \cosh{a}}{\cosh{c}\sinh{b}} $

$\cosh{b_c} = \frac{\cosh{b}\cosh{c}}{\sqrt{2\cosh{a}\cosh{b}\cosh{c} - \cosh^2{c} - \cosh^2{a}}}  $
\end{center}


Next we use the hyperbolic rule of cosines:

\begin{center}
$\frac{\cosh{b}\cosh{c} - \cosh{a}}{\sinh{b}\sinh{c}} = \cos{\alpha} = \frac{\cosh{b_c}\cosh{c_b} - \cosh{a^{*}}}{\sinh{b_c}\sinh{c_b}}$
\end{center}

Expressing $a^{*}$:

\begin{center}
$\cosh{a^{*}} = \cosh{b_c}\cosh{c_b} - \frac{\cosh{b}\cosh{c} - \cosh{a}}{\sinh{b}\sinh{c}}\sinh{b_c}\sinh{c_b} = $

$\cosh{b_c}\cosh{c_b}\left(1 - \frac{\cosh{a}\cosh{c} - \cosh{a}}{\sinh{b}\sinh{c}}\tanh{b_c}\tanh{c_b}\right) = $

$\cosh{b_c}\cosh{c_b}\left(1 - \frac{\cosh{a}\cosh{c} - \cosh{a}}{\sinh{b}\sinh{c}}  \frac{\cosh{c}\cosh{b} - \cosh{a}}{\cosh{b}\sinh{c}} \frac{\cosh{b}\cosh{c} - \cosh{a}}{\cosh{c}\sinh{b}}    \right) =$

$\frac{\cosh{c}\cosh{b}}{\sqrt{2\cosh{a}\cosh{b}\cosh{c} - \cosh^2{b} - \cosh^2{a}}}\frac{\cosh{b}\cosh{c}}{\sqrt{2\cosh{a}\cosh{b}\cosh{c} - \cosh^2{c} - \cosh^2{a}}}\left(1 - \frac{\left(\cosh{b}\cosh{c} - \cosh{a}\right)^3  }{\cosh{b}\cosh{c}\sinh^2{b}\sinh^2{c}}\right) =$

$\frac{\cosh{c}\cosh{b}}{\sqrt{2\cosh{a}\cosh{b}\cosh{c} - \cosh^2{b} - \cosh^2{a}}}\frac{\cosh{b}\cosh{c}}{\sqrt{2\cosh{a}\cosh{b}\cosh{c} - \cosh^2{c} - \cosh^2{a}}}\left(1 - \frac{\left(\cosh{b}\cosh{c} - \cosh{a}\right)^3  }{\cosh{b}\cosh{c}\sinh^2{b}\sinh^2{c}}\right) =$


$\frac{\cosh{c}\cosh{b}\left(\cosh{c}\cosh{b} - \frac{\left(\cosh{b}\cosh{c} - \cosh{a}\right)^3}{\sinh^2{b}\sinh^2{c}}\right)}{\sqrt{\left(2\cosh{a}\cosh{b}\cosh{c} - \cosh^2{b} - \cosh^2{a}\right)\left(2\cosh{a}\cosh{b}\cosh{c} - \cosh^2{c} - \cosh^2{a}\right)}} =$

$\frac{\cosh{c}\cosh{b}\left(\cosh{c}\cosh{b} - \frac{\left(\cosh{b}\cosh{c} - \cosh{a}\right)^3}{ \left( \cosh^2{b}-1\right)\left(\cosh^2{c} -1\right) }\right)}{\sqrt{\left(2\cosh{a}\cosh{b}\cosh{c} - \cosh^2{b} - \cosh^2{a}\right)\left(2\cosh{a}\cosh{b}\cosh{c} - \cosh^2{c} - \cosh^2{a}\right)}} =$

\end{center}







\end{document}



